Coq/adaptation.v
@@ -1,0 +1,394 @@
+Require Import common.
+Require Import loo_def.
+Require Import loo_properties.
+Require Import function_operations.
+Require Import List.
+Require Import CpdtTactics.
+Require Import Coq.Logic.FunctionalExtensionality.
+
+Lemma reduction_implies_stack_head1 :
+  forall M σ1 σ2, M ∙ σ1 ⤳ σ2 ->
+             exists χ ϕ ψ, σ1 = (χ, ϕ :: ψ).
+Proof.
+  intros.
+  inversion H;
+    eauto.
+Qed.
+
+Lemma reduction_implies_stack_head2 :
+  forall M σ1 σ2, M ∙ σ1 ⤳ σ2 ->
+             exists χ ϕ ψ, σ2 = (χ, ϕ :: ψ).
+Proof.
+  intros.
+  inversion H;
+    eauto.
+Qed.
+
+Lemma internal_reductions_implies_stack_head1 :
+  forall M1 M2 σ1 σ2, M1 ⦂ M2 ⦿ σ1 ⤳… σ2 ->
+                 exists χ ϕ ψ, σ1 = (χ, ϕ :: ψ).
+Proof.
+  intros.
+  induction H;
+    subst;
+    eauto.
+  eapply reduction_implies_stack_head1;
+    eauto.
+Qed.
+                 
+Lemma internal_reduction_implies_stack_head2 :
+  forall M1 M2 σ1 σ2, M1 ⦂ M2 ⦿ σ1 ⤳… σ2 ->
+                 exists χ ϕ ψ, σ2 = (χ, ϕ :: ψ).
+Proof.
+  intros.
+  inversion H;
+    subst;
+    eauto;
+    eapply reduction_implies_stack_head2;
+    eauto.
+Qed.
+                 
+Lemma pair_reduction_implies_stack_head1 :
+  forall M1 M2 σ1 σ2, M1 ⦂ M2 ⦿ σ1 ⤳ σ2 ->
+                 exists χ ϕ ψ, σ1 = (χ, ϕ :: ψ).
+Proof.
+  intros.
+  inversion H;
+    subst;
+    eauto.
+  - eapply internal_reductions_implies_stack_head1;
+      eauto.
+  - eapply reduction_implies_stack_head1;
+      eauto.
+Qed.
+                 
+Lemma pair_reduction_implies_stack_head2 :
+  forall M1 M2 σ1 σ2, M1 ⦂ M2 ⦿ σ1 ⤳ σ2 ->
+                 exists χ ϕ ψ, σ2 = (χ, ϕ :: ψ).
+Proof.
+  intros.
+  inversion H;
+    subst;
+    eauto;
+    eapply reduction_implies_stack_head2;
+    eauto.
+Qed.
+                 
+Lemma pair_reductions_implies_stack_head1 :
+  forall M1 M2 σ1 σ2, M1 ⦂ M2 ⦿ σ1 ⤳⋆ σ2 ->
+                 exists χ ϕ ψ, σ1 = (χ, ϕ :: ψ).
+Proof.
+  intros.
+  induction H;
+    subst;
+    eauto.
+  - eapply pair_reduction_implies_stack_head1;
+      eauto.
+Qed.
+                 
+Lemma pair_reductions_implies_stack_head2 :
+  forall M1 M2 σ1 σ2, M1 ⦂ M2 ⦿ σ1 ⤳⋆ σ2 ->
+                 exists χ ϕ ψ, σ2 = (χ, ϕ :: ψ).
+Proof.
+  intros.
+  inversion H;
+    subst;
+    eapply pair_reduction_implies_stack_head2;
+    eauto.
+Qed.
+
+Lemma adapted_mapping_var :
+  forall σ (x : var) o, mapp σ x = o ->
+                   forall χ ϕ ψ, σ = (χ, ϕ :: ψ) ->
+                            forall ψ', mapp (σ ◁ ψ') x = o.
+Proof.
+  intro σ;
+    intros;
+    subst.
+  unfold stack_append in *;
+    simpl in *.
+  repeat map_rewrite;
+    simpl in *.
+  auto.
+Qed.
+
+Lemma adapted_mapping_addr :
+  forall σ (α : addr) o, mapp σ α = o ->
+                   forall χ ϕ ψ, σ = (χ, ϕ :: ψ) ->
+                            forall ψ', mapp (σ ◁ ψ') α = o.
+Proof.
+  intro σ;
+    intros;
+    subst.
+  unfold stack_append in *;
+    simpl in *.
+  repeat map_rewrite;
+    simpl in *.
+  auto.
+Qed.
+
+Lemma adapted_interpretation :
+  forall σ x v, ⌊ x ⌋ σ ≜ v ->
+           forall χ ϕ ψ, σ = (χ, ϕ :: ψ) ->
+                    forall ψ', ⌊ x ⌋ (σ ◁ ψ') ≜ v.
+Proof.
+  intros;
+    subst;
+    apply int_x.
+  eapply adapted_mapping_var;
+    eauto.
+  match goal with
+  | [H : ⌊ _ ⌋ _ ≜ _ |- _] =>
+    inversion H;
+      subst;
+      auto
+  end.
+Qed.
+
+Hint Resolve adapted_mapping_var adapted_mapping_addr adapted_interpretation : loo_db.
+Hint Rewrite adapted_mapping_var adapted_mapping_addr adapted_interpretation : loo_db.
+
+Lemma adapted_update_σ_map :
+  forall χ ϕ ψ ψ' x v, update_σ_map ((χ, ϕ :: ψ) ◁ ψ') x v =
+                  (update_σ_map (χ, ϕ :: ψ) x v) ◁ ψ'.
+Proof.
+  intros.
+  unfold stack_append.
+  repeat map_rewrite;
+    simpl;
+    auto.
+Qed.
+
+Lemma adapted_evaluation :
+  forall M σ e v, M ∙ σ ⊢ e ↪ v ->
+             forall χ ϕ ψ, σ = (χ, ϕ :: ψ) ->
+                      forall ψ', M ∙ (σ ◁ ψ') ⊢ e ↪ v.
+Proof.
+  intros M σ e v Heval;
+    induction Heval;
+    intros;
+    subst;
+    eauto with loo_db.
+
+  - eapply v_f_ghost;
+      eauto.
+
+    unfold update_σ_map in *; simpl in *.
+    unfold stack_append in *; simpl in *.
+    eauto.
+Qed.
+
+Lemma adapted_classOf :
+  forall x σ C, classOf x σ C ->
+           forall χ ϕ ψ ψ', σ = (χ, ϕ :: ψ) ->
+                       classOf x (σ ◁ ψ') C.
+Proof.
+  intros;
+    subst.
+  inversion H;
+    subst;
+    unfold stack_append;
+    simpl in *.
+  eapply adapted_interpretation with (ψ':=ψ') in H0;
+    eauto.
+  eapply cls_of;
+    eauto.
+Qed.
+
+Lemma adapted_reduction :
+  forall M σ1 σ2, M ∙ σ1 ⤳ σ2 ->
+             forall ψ, M ∙ (σ1 ◁ ψ) ⤳ (σ2 ◁ ψ).
+Proof.
+  intros M σ1 σ2 Hred;
+    induction Hred;
+    intros;
+    subst;
+    repeat match goal with
+           | [H : classOf _ (_ , _ :: _) _ |- context[_ ◁ ?ψ]] =>
+             eapply adapted_classOf with (ψ':=ψ) in H;
+               eauto
+           end;
+    repeat match goal with
+           | [H : _ ∙ (_ , _ :: _) ⊢ _ ↪ _ |- context[_ ◁ ?ψ]] =>
+             eapply adapted_evaluation with (ψ':=ψ) in H;
+               eauto
+           end;
+    repeat match goal with
+           | [H : ⌊ _ ⌋ (_ , _ :: _) ≜ _ |- context[_ ◁ ?ψ]] =>
+             eapply adapted_interpretation with (ψ':=ψ) in H;
+               eauto
+           end;  
+    unfold stack_append in *;
+    simpl in *;
+    try solve [eapply r_mth; eauto];
+    try solve [eapply r_new; eauto];
+    try solve [eauto with loo_db].
+Qed.
+
+Lemma adapted_is_internal :
+  forall M1 M2 σ x, is_internal M1 M2 σ x ->
+               forall ψ, is_internal M1 M2 (σ ◁ ψ) x.
+Proof.
+  intros;
+    unfold is_internal in *;
+    intros;
+    repeat destruct_exists_loo;
+    andDestruct;
+    subst.
+  destruct σ as [χ ψ'].
+  assert (exists ϕ ψ'', ψ' = ϕ :: ψ'');
+  [|repeat destruct_exists_loo; subst].
+  + destruct ψ' as [|ϕ ψ''];
+      [|eauto].
+    repeat map_rewrite;
+      crush.
+  + repeat match goal with
+           | [H : mapp (_, _ :: _) _ = _ |- context[_ ◁ ?ψ]] =>
+             try (eapply adapted_mapping_addr with (ψ':=ψ) in H);
+               try (eapply adapted_mapping_var with (ψ':=ψ) in H);
+               eauto
+           end.
+    repeat eexists; eauto.
+Qed.
+
+Lemma adapted_is_external :
+  forall M1 M2 σ x, is_external M1 M2 σ x ->
+               forall ψ, is_external M1 M2 (σ ◁ ψ) x.
+Proof.
+  intros;
+    unfold is_external in *;
+    intros;
+    repeat destruct_exists_loo;
+    andDestruct;
+    subst.
+  destruct σ as [χ ψ'].
+  assert (exists ϕ ψ'', ψ' = ϕ :: ψ'');
+  [|repeat destruct_exists_loo; subst].
+  + destruct ψ' as [|ϕ ψ''];
+      [|eauto].
+    repeat map_rewrite;
+      crush.
+  + repeat match goal with
+         | [H : mapp (_, _ :: _) _ = _ |- context[_ ◁ ?ψ]] =>
+           try (eapply adapted_mapping_addr with (ψ':=ψ) in H);
+           try (eapply adapted_mapping_var with (ψ':=ψ) in H);
+             eauto
+         end.
+Qed.
+
+Lemma adapted_internal_self :
+  forall M1 M2 σ, internal_self M1 M2 σ ->
+             forall ψ, internal_self M1 M2 (σ ◁ ψ).
+Proof.
+  intros;
+    unfold internal_self in *;
+    intros;
+    subst.
+  eapply adapted_is_internal; eauto.
+Qed.
+
+Lemma adapted_external_self :
+  forall M1 M2 σ, external_self M1 M2 σ ->
+             forall ψ, external_self M1 M2 (σ ◁ ψ).
+Proof.
+  intros;
+    unfold external_self in *;
+    intros;
+    subst.
+  eapply adapted_is_external;
+    eauto.
+Qed.
+
+Lemma adapted_internal_reductions :
+  forall M1 M2 σ1 σ2, M1 ⦂ M2 ⦿ σ1 ⤳… σ2 ->
+                 forall ψ, M1 ⦂ M2 ⦿ (σ1 ◁ ψ) ⤳… (σ2 ◁ ψ).
+Proof.
+  intros M1 M2 σ1 σ2 Hred;
+    induction Hred;
+    intros;
+    subst;
+    try match goal with
+        | [H : ?M ∙ ?σ1 ⤳ ?σ2 |- context[_ ◁ ?ψ']] =>
+          notHyp (M ∙ σ1 ◁ ψ' ⤳ (σ2 ◁ ψ'));
+            eapply adapted_reduction with (ψ':=ψ') in H;
+            eauto
+        end;
+    try match goal with
+        | [H : internal_self _ _ _ |- context[_ ◁ ?ψ']] =>
+          eapply adapted_internal_self with (ψ:=ψ') in H;
+            eauto
+        end;
+    try match goal with
+        | [H : external_self _ _ _ |- context[_ ◁ ?ψ']] =>
+          eapply adapted_external_self with (ψ:=ψ') in H;
+            eauto
+        end.
+
+  - eapply pr_single; eauto.
+
+  - eapply pr_trans; eauto.
+Qed.
+
+Lemma adapted_pair_reduction :
+  forall M1 M2 σ1 σ2, M1 ⦂ M2 ⦿ σ1 ⤳ σ2 ->
+                 forall ψ, M1 ⦂ M2 ⦿ (σ1 ◁ ψ) ⤳ (σ2 ◁ ψ).
+Proof.
+  intros.
+  inversion H;
+    subst;
+    try match goal with
+        | [H : ?M ∙ ?σ1 ⤳ ?σ2 |- context[_ ◁ ?ψ']] =>
+          notHyp (M ∙ σ1 ◁ ψ' ⤳ (σ2 ◁ ψ'));
+            eapply adapted_reduction with (ψ':=ψ') in H;
+            eauto
+        end;
+    try match goal with
+        | [H : ?M1 ⦂ ?M2 ⦿ ?σ1 ⤳… ?σ2 |- context[_ ◁ ?ψ']] =>
+          notHyp (M1 ⦂ M2 ⦿ σ1 ◁ ψ' ⤳… (σ2 ◁ ψ'));
+            eapply adapted_internal_reductions with (ψ':=ψ') in H;
+            eauto
+        end;
+    try match goal with
+        | [H : internal_self _ _ _ |- context[_ ◁ ?ψ']] =>
+          eapply adapted_internal_self with (ψ:=ψ') in H;
+            eauto
+        end;
+    try match goal with
+        | [H : external_self _ _ _ |- context[_ ◁ ?ψ']] =>
+          eapply adapted_external_self with (ψ:=ψ') in H;
+            eauto
+        end.
+  - eapply p_internal;
+      eauto.
+  - eapply p_external;
+      eauto.
+    eapply adapted_external_self; eauto.
+Qed.
+
+Lemma adapted_pair_reductions :
+  forall M1 M2 σ1 σ2, M1 ⦂ M2 ⦿ σ1 ⤳⋆ σ2 ->
+                 forall ψ, M1 ⦂ M2 ⦿ (σ1 ◁ ψ) ⤳⋆ (σ2 ◁ ψ).
+Proof.
+  intros;
+    induction H;
+    subst.
+  - eapply prs_single; eauto.
+    eapply adapted_pair_reduction;
+      eauto.
+  - eapply prs_trans; eauto.
+    eapply adapted_pair_reduction;
+      eauto.
+Qed.
+
+Lemma constrained_pair_reduction_is_reduction :
+  forall M1 M2 σ1 σ2, M1 ⦂ M2 ⦿ σ1 ⌈⤳⋆⌉ σ2 ->
+                 M1 ⦂ M2 ⦿ σ1 ⤳⋆ σ2.
+Proof.
+  intros.
+  unfold constrained_pair_reductions in *.
+  repeat destruct_exists_loo;
+    andDestruct;
+    subst.
+  apply adapted_pair_reductions with (ψ:=ψ) in Ha0;
+    auto.
+Qed.
